setup project

Project_Tseitin.thy
@@ -11,7 +11,7 @@ into equisatisfiable CNFs and formally prove results about their complexity and 
 the resulting CNFs are indeed equisatisfiable to the original formula.
 \<close>
 
-theory Project_Tseitin
+theory Project_Tseitin 
   imports Main
 begin
 
@@ -89,7 +89,6 @@ fun of_cnf :: "'a cnf \<Rightarrow> 'a form"
   where
     "of_cnf [] = Neg Bot"
   | "of_cnf (c # cs) = Neg (Imp (of_clause c) (Neg (of_cnf cs)))"
-print_theorems
 
 
 subsection \<open>Tseitin Transformation\<close>
@@ -101,7 +100,8 @@ a label \<open>a\<^sub>\<phi>\<close> and use the following definitions
 \<^item> \<open>a\<^sub>\<bottom> \<longleftrightarrow> \<bottom>\<close>
 \<^item> \<open>a\<^sub>\<not>\<^sub>\<phi> \<longleftrightarrow> \<not> \<phi>\<close>
 \<^item> \<open>a\<^sub>\<phi>\<^sub>\<longrightarrow>\<^sub>\<psi> \<longleftrightarrow> \<phi> \<longrightarrow> \<psi>\<close>
-
+\<close>
+text \<open>
 to recursively compute clauses \<open>tseitin \<phi>\<close> such that \<open>a\<^sub>\<phi> \<and> tseitin \<phi>\<close> and \<open>\<phi>\<close>
 are equisatisfiable (that is, the former is satisfiable iff the latter is).
 
@@ -112,13 +112,15 @@ fun tseitin :: "'a form \<Rightarrow> ('a form) cnf"
     "tseitin (Bot) = [[N Bot]]"
   | "tseitin (Atm \<phi>) = []"
   | "tseitin (Neg \<phi>) = [(N (Neg \<phi>)), (N \<phi>)] # [(P (Neg \<phi>)), (P \<phi>)] # tseitin \<phi>"
-  | "tseitin (Imp \<phi> \<psi>) = [(N (Imp \<phi> \<psi>)), (N \<phi>), (P \<psi>)] # [(P (Imp \<phi> \<psi>)), (P \<phi>)] 
-                         # [(N \<psi>), (P (Imp \<phi> \<psi>))] # (tseitin \<phi> @ tseitin \<psi>)"
+  | "tseitin (Imp \<phi> \<psi>) 
+    = [(N (Imp \<phi> \<psi>)), (N \<phi>), (P \<psi>)] # [(P (Imp \<phi> \<psi>)), (P \<phi>)] 
+    # [(N \<psi>), (P (Imp \<phi> \<psi>))] # (tseitin \<phi> @ tseitin \<psi>)"
 
 text \<open>
-We prove that the evaluation of the function {@const of_cnf} preserves list concatenation.
+We prove that the evaluation of the function @{const of_cnf} preserves list concatenation.
 \<close>
-lemma cnf_linear [simp]: "eval \<alpha> (of_cnf (xs @ ys)) = (eval \<alpha> (of_cnf xs) \<and> eval \<alpha> (of_cnf ys))"
+lemma cnf_linear [simp]: 
+  "eval \<alpha> (of_cnf (xs @ ys)) = (eval \<alpha> (of_cnf xs) \<and> eval \<alpha> (of_cnf ys))"
   by (induction xs) auto
 
 text 
@@ -153,7 +155,8 @@ next
   then show ?case using IH by auto
 next
   case IH: (Imp \<phi>1 \<phi>2)
-  then have 1: "eval v (of_cnf (tseitin \<phi>1)) \<and> eval v (of_cnf (tseitin \<phi>2))" by auto
+  then have 1: "eval v (of_cnf (tseitin \<phi>1)) \<and> eval v (of_cnf (tseitin \<phi>2))" 
+    by auto
   from 1 have 2: "eval v (of_cnf (tseitin \<phi>1))" by auto
   from 1 have 3: "eval v (of_cnf (tseitin \<phi>2))" by auto
   from \<open>eval v (of_cnf (tseitin \<phi>1)) \<Longrightarrow> eval (v \<circ> Atm) \<phi>1 = v \<phi>1\<close> 
@@ -208,10 +211,10 @@ fun num_literals :: "('a form) cnf \<Rightarrow> nat"
   | "num_literals (c # cs) = length c + num_literals cs"
 
 text \<open>
-We show that the function {@const num_literals} preserves list concatenation:
+We show that the function @{const num_literals} preserves list concatenation:
 \<close>
 lemma num_literals_add [simp]:
-"num_literals (xs @ ys) = num_literals xs + num_literals ys"
+  "num_literals (xs @ ys) = num_literals xs + num_literals ys"
   by (induction xs) auto
 
 text \<open>
@@ -231,7 +234,6 @@ fun t_tseitin :: "'a form \<Rightarrow> nat"
   | "t_tseitin (Atm \<phi>) = 0"
   | "t_tseitin (Neg \<phi>) = 1 + t_tseitin \<phi>"
   | "t_tseitin (Imp \<phi> \<psi>) = 2 + t_tseitin \<phi> + t_tseitin \<psi>"
-print_theorems
 
 lemma tseitin_linear:
   "t_tseitin \<phi> \<le> 2 * size \<phi>"
@@ -245,10 +247,10 @@ fun tseitin2 :: "'a form \<Rightarrow> ('a form) cnf \<Rightarrow> ('a form) cnf
     "tseitin2 Bot acc = ([N Bot] # acc)"
   | "tseitin2 (Atm \<phi>) acc = acc"
   | "tseitin2 (Neg \<phi>) acc
-          = tseitin2 \<phi> ([(N (Neg \<phi>)), (N \<phi>)] # [(P (Neg \<phi>)), (P \<phi>)] # acc)"
+    = tseitin2 \<phi> ([(N (Neg \<phi>)), (N \<phi>)] # [(P (Neg \<phi>)), (P \<phi>)] # acc)"
   | "tseitin2 (Imp \<phi> \<psi>) acc
-          = tseitin2 \<psi> (tseitin2 \<phi> ([(N (Imp \<phi> \<psi>)), (N \<phi>), (P \<psi>)] # [(P (Imp \<phi> \<psi>)), (P \<phi>)] 
-                         # [(N \<psi>), (P (Imp \<phi> \<psi>))] # acc))"
+    = tseitin2 \<psi> (tseitin2 \<phi> ([(N (Imp \<phi> \<psi>)), (N \<phi>), (P \<psi>)] 
+    # [(P (Imp \<phi> \<psi>)), (P \<phi>)] # [(N \<psi>), (P (Imp \<phi> \<psi>))] # acc))"
 
 text \<open>
 We show that we can also append the accumulator instead of using it as an argument
@@ -264,17 +266,23 @@ next
 next
   case (Neg \<phi>)
   then have 1: "\<forall>acc. tseitin2 \<phi> acc = tseitin2 \<phi> [] @ acc" by (rule allI)
-  have 2: "tseitin2 (Neg \<phi>) acc = tseitin2 \<phi> ([(N (Neg \<phi>)), (N \<phi>)] # [(P (Neg \<phi>)), (P \<phi>)] # acc)"
+  have 2: "tseitin2 (Neg \<phi>) acc 
+    = tseitin2 \<phi> ([(N (Neg \<phi>)), (N \<phi>)] # [(P (Neg \<phi>)), (P \<phi>)] # acc)"
     by auto
-  from 1 have 3: "tseitin2 \<phi> ([(N (Neg \<phi>)), (N \<phi>)] # [(P (Neg \<phi>)), (P \<phi>)] # acc)
-          = (tseitin2 \<phi> []) @ [(N (Neg \<phi>)), (N \<phi>)] # [(P (Neg \<phi>)), (P \<phi>)] # acc" by (rule allE)
-  also have 4: "...
-          = ((tseitin2 \<phi> []) @ [(N (Neg \<phi>)), (N \<phi>)] # [[(P (Neg \<phi>)), (P \<phi>)]]) @ acc" by auto
-  from 1 have 5: "(tseitin2 \<phi> ([(N (Neg \<phi>)), (N \<phi>)] # [[(P (Neg \<phi>)), (P \<phi>)]])) 
-          = ((tseitin2 \<phi> []) @ [(N (Neg \<phi>)), (N \<phi>)] # [[(P (Neg \<phi>)), (P \<phi>)]])" 
+  from 1 have 3: 
+    "tseitin2 \<phi> ([(N (Neg \<phi>)), (N \<phi>)] # [(P (Neg \<phi>)), (P \<phi>)] # acc)
+    = (tseitin2 \<phi> []) @ [(N (Neg \<phi>)), (N \<phi>)] # [(P (Neg \<phi>)), (P \<phi>)] # acc" 
     by (rule allE)
-  from this have "((tseitin2 \<phi> []) @ [(N (Neg \<phi>)), (N \<phi>)] # [[(P (Neg \<phi>)), (P \<phi>)]])
-          = (tseitin2 \<phi> ([(N (Neg \<phi>)), (N \<phi>)] # [[(P (Neg \<phi>)), (P \<phi>)]]))" by (rule sym)
+  also have 4: "...
+    = ((tseitin2 \<phi> []) @ [(N (Neg \<phi>)), (N \<phi>)] # [[(P (Neg \<phi>)), (P \<phi>)]]) @ acc" 
+    by auto
+  from 1 have 5: "(tseitin2 \<phi> ([(N (Neg \<phi>)), (N \<phi>)] # [[(P (Neg \<phi>)), (P \<phi>)]])) 
+    = ((tseitin2 \<phi> []) @ [(N (Neg \<phi>)), (N \<phi>)] # [[(P (Neg \<phi>)), (P \<phi>)]])" 
+    by (rule allE)
+  from this have 
+    "((tseitin2 \<phi> []) @ [(N (Neg \<phi>)), (N \<phi>)] # [[(P (Neg \<phi>)), (P \<phi>)]]) 
+    = (tseitin2 \<phi> ([(N (Neg \<phi>)), (N \<phi>)] # [[(P (Neg \<phi>)), (P \<phi>)]]))" 
+    by (rule sym)
   from 2 and 3 and 4 and this show ?case by auto
 next
   case IH: (Imp \<phi> \<psi>)
@@ -282,54 +290,64 @@ next
   have 1: "\<forall>acc. tseitin2 \<phi> acc = tseitin2 \<phi> [] @ acc" by (rule allI)
   from \<open>\<And>acc. (tseitin2 \<psi> acc = tseitin2 \<psi> [] @ acc)\<close>
   have 2: "\<forall>acc. tseitin2 \<psi> acc = tseitin2 \<psi> [] @ acc" by (rule allI)
-  from 2 have 3: "tseitin2 \<psi> (tseitin2 \<phi> ([(N (Imp \<phi> \<psi>)), (N \<phi>), (P \<psi>)] # [(P (Imp \<phi> \<psi>)), (P \<phi>)] 
-                         # [(N \<psi>), (P (Imp \<phi> \<psi>))] # acc))
-          = tseitin2 \<psi> [] @ (tseitin2 \<phi> ([(N (Imp \<phi> \<psi>)), (N \<phi>), (P \<psi>)] # [(P (Imp \<phi> \<psi>)), (P \<phi>)] 
-                         # [(N \<psi>), (P (Imp \<phi> \<psi>))] # acc))" by (rule allE)
+  from 2 have 3: 
+    "tseitin2 \<psi> (tseitin2 \<phi> ([(N (Imp \<phi> \<psi>)), (N \<phi>), (P \<psi>)] 
+    # [(P (Imp \<phi> \<psi>)), (P \<phi>)] # [(N \<psi>), (P (Imp \<phi> \<psi>))] # acc))
+    = tseitin2 \<psi> [] @ (tseitin2 \<phi> ([(N (Imp \<phi> \<psi>)), (N \<phi>), (P \<psi>)] 
+    # [(P (Imp \<phi> \<psi>)), (P \<phi>)] # [(N \<psi>), (P (Imp \<phi> \<psi>))] # acc))" 
+    by (rule allE)
   from 1 have 4: 
-           "tseitin2 \<phi> ([(N (Imp \<phi> \<psi>)), (N \<phi>), (P \<psi>)] # [(P (Imp \<phi> \<psi>)), (P \<phi>)] 
-                         # [(N \<psi>), (P (Imp \<phi> \<psi>))] # acc)
-          = tseitin2 \<phi> [] @ [(N (Imp \<phi> \<psi>)), (N \<phi>), (P \<psi>)] # [(P (Imp \<phi> \<psi>)), (P \<phi>)] 
-                         # [(N \<psi>), (P (Imp \<phi> \<psi>))] # acc" by (rule allE)
+    "tseitin2 \<phi> ([(N (Imp \<phi> \<psi>)), (N \<phi>), (P \<psi>)] # [(P (Imp \<phi> \<psi>)), (P \<phi>)] 
+    # [(N \<psi>), (P (Imp \<phi> \<psi>))] # acc)
+    = tseitin2 \<phi> [] @ [(N (Imp \<phi> \<psi>)), (N \<phi>), (P \<psi>)] # [(P (Imp \<phi> \<psi>)), (P \<phi>)] 
+    # [(N \<psi>), (P (Imp \<phi> \<psi>))] # acc" 
+    by (rule allE)
   then have 5: 
-           "tseitin2 \<psi> [] @ tseitin2 \<phi> ([(N (Imp \<phi> \<psi>)), (N \<phi>), (P \<psi>)] # [(P (Imp \<phi> \<psi>)), (P \<phi>)] 
-                         # [(N \<psi>), (P (Imp \<phi> \<psi>))] # acc)
-          = tseitin2 \<psi> [] @ tseitin2 \<phi> [] @ [(N (Imp \<phi> \<psi>)), (N \<phi>), (P \<psi>)] # [(P (Imp \<phi> \<psi>)), (P \<phi>)] 
-                         # [(N \<psi>), (P (Imp \<phi> \<psi>))] # acc" by auto
+    "tseitin2 \<psi> [] @ tseitin2 \<phi> ([(N (Imp \<phi> \<psi>)), (N \<phi>), (P \<psi>)] 
+    # [(P (Imp \<phi> \<psi>)), (P \<phi>)] # [(N \<psi>), (P (Imp \<phi> \<psi>))] # acc)
+    = tseitin2 \<psi> [] @ tseitin2 \<phi> [] @ [(N (Imp \<phi> \<psi>)), (N \<phi>), (P \<psi>)] 
+    # [(P (Imp \<phi> \<psi>)), (P \<phi>)] # [(N \<psi>), (P (Imp \<phi> \<psi>))] # acc" 
+    by auto
   from 1 have 6:
-           "tseitin2 \<phi> ([(N (Imp \<phi> \<psi>)), (N \<phi>), (P \<psi>)] # [(P (Imp \<phi> \<psi>)), (P \<phi>)] 
-                         # [[(N \<psi>), (P (Imp \<phi> \<psi>))]])
-          = tseitin2 \<phi> [] @ [(N (Imp \<phi> \<psi>)), (N \<phi>), (P \<psi>)] # [(P (Imp \<phi> \<psi>)), (P \<phi>)] 
-                         # [[(N \<psi>), (P (Imp \<phi> \<psi>))]]" by (rule allE)
+    "tseitin2 \<phi> ([(N (Imp \<phi> \<psi>)), (N \<phi>), (P \<psi>)] # [(P (Imp \<phi> \<psi>)), (P \<phi>)] 
+    # [[(N \<psi>), (P (Imp \<phi> \<psi>))]])
+    = tseitin2 \<phi> [] @ [(N (Imp \<phi> \<psi>)), (N \<phi>), (P \<psi>)] # [(P (Imp \<phi> \<psi>)), (P \<phi>)] 
+    # [[(N \<psi>), (P (Imp \<phi> \<psi>))]]" 
+    by (rule allE)
   then have 7:
-           "tseitin2 \<phi> [] @ [(N (Imp \<phi> \<psi>)), (N \<phi>), (P \<psi>)] # [(P (Imp \<phi> \<psi>)), (P \<phi>)] 
-                         # [[(N \<psi>), (P (Imp \<phi> \<psi>))]] 
-          = tseitin2 \<phi> ([(N (Imp \<phi> \<psi>)), (N \<phi>), (P \<psi>)] # [(P (Imp \<phi> \<psi>)), (P \<phi>)] 
-                         # [[(N \<psi>), (P (Imp \<phi> \<psi>))]])" by (rule sym)
+    "tseitin2 \<phi> [] @ [(N (Imp \<phi> \<psi>)), (N \<phi>), (P \<psi>)] # [(P (Imp \<phi> \<psi>)), (P \<phi>)] 
+    # [[(N \<psi>), (P (Imp \<phi> \<psi>))]] 
+    = tseitin2 \<phi> ([(N (Imp \<phi> \<psi>)), (N \<phi>), (P \<psi>)] # [(P (Imp \<phi> \<psi>)), (P \<phi>)] 
+    # [[(N \<psi>), (P (Imp \<phi> \<psi>))]])" 
+    by (rule sym)
   from 2 have 8:
-           "tseitin2 \<psi> (tseitin2 \<phi> ([(N (Imp \<phi> \<psi>)), (N \<phi>), (P \<psi>)] # [(P (Imp \<phi> \<psi>)), (P \<phi>)] 
-                         # [[(N \<psi>), (P (Imp \<phi> \<psi>))]]))
-          = tseitin2 \<psi> [] @ tseitin2 \<phi> ([(N (Imp \<phi> \<psi>)), (N \<phi>), (P \<psi>)] # [(P (Imp \<phi> \<psi>)), (P \<phi>)] 
-                         # [[(N \<psi>), (P (Imp \<phi> \<psi>))]])" by (rule allE)
+    "tseitin2 \<psi> (tseitin2 \<phi> ([(N (Imp \<phi> \<psi>)), (N \<phi>), (P \<psi>)] 
+    # [(P (Imp \<phi> \<psi>)), (P \<phi>)] # [[(N \<psi>), (P (Imp \<phi> \<psi>))]]))
+    = tseitin2 \<psi> [] @ tseitin2 \<phi> ([(N (Imp \<phi> \<psi>)), (N \<phi>), (P \<psi>)] 
+    # [(P (Imp \<phi> \<psi>)), (P \<phi>)] # [[(N \<psi>), (P (Imp \<phi> \<psi>))]])" 
+    by (rule allE)
   then have 9:
-           "tseitin2 \<psi> [] @ tseitin2 \<phi> ([(N (Imp \<phi> \<psi>)), (N \<phi>), (P \<psi>)] # [(P (Imp \<phi> \<psi>)), (P \<phi>)] 
-                         # [[(N \<psi>), (P (Imp \<phi> \<psi>))]])
-          = tseitin2 \<psi> (tseitin2 \<phi> ([(N (Imp \<phi> \<psi>)), (N \<phi>), (P \<psi>)] # [(P (Imp \<phi> \<psi>)), (P \<phi>)] 
-                         # [[(N \<psi>), (P (Imp \<phi> \<psi>))]]))" by (rule sym)
+    "tseitin2 \<psi> [] @ tseitin2 \<phi> ([(N (Imp \<phi> \<psi>)), (N \<phi>), (P \<psi>)] 
+    # [(P (Imp \<phi> \<psi>)), (P \<phi>)] # [[(N \<psi>), (P (Imp \<phi> \<psi>))]])
+    = tseitin2 \<psi> (tseitin2 \<phi> ([(N (Imp \<phi> \<psi>)), (N \<phi>), (P \<psi>)] 
+    # [(P (Imp \<phi> \<psi>)), (P \<phi>)] # [[(N \<psi>), (P (Imp \<phi> \<psi>))]]))" 
+    by (rule sym)
   from 3 and 5 and 7 and 9 show ?case by auto
 qed
 
 text \<open>
 And we prove the symmetric case of the lemma above.
 \<close>
-lemma tseitin2_concat2: "tseitin2 \<phi> [] @ acc = tseitin2 \<phi> acc"  
+lemma tseitin2_concat2: 
+  "tseitin2 \<phi> [] @ acc = tseitin2 \<phi> acc"  
   by (rule sym, rule tseitin2_concat)
 
 text \<open>
 In the following lemma, we prove that the evaluation of {@const tseitin} is the same as the 
 evaluation of the {@const tseitin2} using tail recursion technique.
 \<close>
-lemma tseitin_equality: "eval \<alpha> (of_cnf(tseitin \<phi>)) \<longleftrightarrow> eval \<alpha> (of_cnf(tseitin2 \<phi> []))"
+lemma tseitin_equality: 
+  "eval \<alpha> (of_cnf(tseitin \<phi>)) \<longleftrightarrow> eval \<alpha> (of_cnf(tseitin2 \<phi> []))"
 proof (induction \<phi>)
   case Bot
   show ?case by auto
@@ -339,44 +357,57 @@ next
 next
   case IH: (Neg \<phi>)
   have "eval \<alpha> (of_cnf(tseitin (Neg \<phi>))) = (eval \<alpha> (of_cnf(tseitin \<phi>)) 
-        \<and> eval \<alpha> (of_cnf([(N (Neg \<phi>)), (N \<phi>)] # [[(P (Neg \<phi>)), (P \<phi>)]])))" by auto
+    \<and> eval \<alpha> (of_cnf([(N (Neg \<phi>)), (N \<phi>)] # [[(P (Neg \<phi>)), (P \<phi>)]])))" 
+    by auto
   also have "... = (eval \<alpha> (of_cnf(tseitin2 \<phi> [])) 
-        \<and> eval \<alpha> (of_cnf([(N (Neg \<phi>)), (N \<phi>)] # [[(P (Neg \<phi>)), (P \<phi>)]])))" unfolding IH ..
-  also have "... = eval \<alpha> (of_cnf(tseitin2 \<phi> [] @ [(N (Neg \<phi>)), (N \<phi>)] # [[(P (Neg \<phi>)), (P \<phi>)]]))"
+    \<and> eval \<alpha> (of_cnf([(N (Neg \<phi>)), (N \<phi>)] # [[(P (Neg \<phi>)), (P \<phi>)]])))" 
+    unfolding IH ..
+  also have "... 
+    = eval \<alpha> (of_cnf(tseitin2 \<phi> [] @ [(N (Neg \<phi>)), (N \<phi>)] 
+    # [[(P (Neg \<phi>)), (P \<phi>)]]))"
     unfolding cnf_linear ..
-  also have "... = eval \<alpha> (of_cnf(tseitin2 \<phi> ([(N (Neg \<phi>)), (N \<phi>)] # [[(P (Neg \<phi>)), (P \<phi>)]])))"
+  also have "... 
+    = eval \<alpha> (of_cnf(tseitin2 \<phi> ([(N (Neg \<phi>)), (N \<phi>)] 
+    # [[(P (Neg \<phi>)), (P \<phi>)]])))"
     unfolding tseitin2_concat2 ..
-  also have "... = eval \<alpha> (of_cnf(tseitin2 (Neg \<phi>) []))" unfolding tseitin2.simps ..
+  also have "... = eval \<alpha> (of_cnf(tseitin2 (Neg \<phi>) []))" 
+    unfolding tseitin2.simps ..
   finally show ?case .
 next
   case IH: (Imp \<phi> \<psi>)
   have "eval \<alpha> (of_cnf(tseitin (Imp \<phi> \<psi>)))
-          = eval \<alpha> (of_cnf (tseitin \<psi> @ tseitin \<phi> 
-          @ ([[(N (Imp \<phi> \<psi>)), (N \<phi>), (P \<psi>)], [(P (Imp \<phi> \<psi>)), (P \<phi>)],
-                         [(N \<psi>), (P (Imp \<phi> \<psi>))]])))" by auto
+    = eval \<alpha> (of_cnf (tseitin \<psi> @ tseitin \<phi> 
+    @ ([[(N (Imp \<phi> \<psi>)), (N \<phi>), (P \<psi>)], [(P (Imp \<phi> \<psi>)), (P \<phi>)],
+    [(N \<psi>), (P (Imp \<phi> \<psi>))]])))" 
+    by auto
   also have "... = eval \<alpha> (of_cnf (tseitin2 \<psi> [] @ tseitin2 \<phi> []
-          @ ([[(N (Imp \<phi> \<psi>)), (N \<phi>), (P \<psi>)], [(P (Imp \<phi> \<psi>)), (P \<phi>)],
-                         [(N \<psi>), (P (Imp \<phi> \<psi>))]])))" using IH by auto
+    @ ([[(N (Imp \<phi> \<psi>)), (N \<phi>), (P \<psi>)], [(P (Imp \<phi> \<psi>)), (P \<phi>)],
+    [(N \<psi>), (P (Imp \<phi> \<psi>))]])))" 
+    using IH by auto
   also have "... = eval \<alpha> (of_cnf (tseitin2 \<psi> []
-          @ (tseitin2 \<phi> ([[(N (Imp \<phi> \<psi>)), (N \<phi>), (P \<psi>)], [(P (Imp \<phi> \<psi>)), (P \<phi>)],
-                         [(N \<psi>), (P (Imp \<phi> \<psi>))]]))))" unfolding tseitin2_concat2 ..
+    @ (tseitin2 \<phi> ([[(N (Imp \<phi> \<psi>)), (N \<phi>), (P \<psi>)], [(P (Imp \<phi> \<psi>)), (P \<phi>)],
+    [(N \<psi>), (P (Imp \<phi> \<psi>))]]))))" 
+    unfolding tseitin2_concat2 ..
   also have "... = eval \<alpha> (of_cnf 
-          (tseitin2 \<psi> (tseitin2 \<phi> ([[(N (Imp \<phi> \<psi>)), (N \<phi>), (P \<psi>)], [(P (Imp \<phi> \<psi>)), (P \<phi>)],
-                         [(N \<psi>), (P (Imp \<phi> \<psi>))]]))))" unfolding tseitin2_concat2 ..
+    (tseitin2 \<psi> (tseitin2 \<phi> ([[(N (Imp \<phi> \<psi>)), (N \<phi>), (P \<psi>)], 
+    [(P (Imp \<phi> \<psi>)), (P \<phi>)], [(N \<psi>), (P (Imp \<phi> \<psi>))]]))))" 
+    unfolding tseitin2_concat2 ..
   finally show ?case by auto
 qed
 
 text \<open>
 And we prove the symmetric case of the lemma above.
 \<close>
-lemma tseitin_equality2: "eval \<alpha> (of_cnf(tseitin2 \<phi> [])) \<longleftrightarrow> eval \<alpha> (of_cnf(tseitin \<phi>))"
+lemma tseitin_equality2: 
+  "eval \<alpha> (of_cnf(tseitin2 \<phi> [])) \<longleftrightarrow> eval \<alpha> (of_cnf(tseitin \<phi>))"
   by (rule sym, rule tseitin_equality)
 
 text \<open>
 Then, we prove that for all formulas \<open>\<phi>\<close> it holds, that evaluating it by the tseitin 
 transformation, is equivalent to evaluation using the tail recursive transformation:
 \<close>
-lemma tseitin_eq_for_all: "\<forall>\<alpha>. (eval \<alpha> (of_cnf(tseitin2 \<phi> [])) \<longleftrightarrow> eval \<alpha> (of_cnf(tseitin \<phi>)))"
+lemma tseitin_eq_for_all: 
+  "\<forall>\<alpha>. (eval \<alpha> (of_cnf(tseitin2 \<phi> [])) \<longleftrightarrow> eval \<alpha> (of_cnf(tseitin \<phi>)))"
 proof -
   have "\<And>\<alpha>. eval \<alpha> (of_cnf (tseitin2 \<phi> [])) \<longleftrightarrow> eval \<alpha> (of_cnf (tseitin \<phi>))"
     by (rule tseitin_equality2)
@@ -387,7 +418,8 @@ text \<open>
 We then show that the equivalence also holds for the existential quantifier, which is needed later.
 \<close>
 lemma tseitin_eq_ex:
- "(\<exists>\<alpha>. eval \<alpha> (of_cnf ([P \<phi>] # tseitin2 \<phi> []))) \<longleftrightarrow> (\<exists>\<alpha>. eval \<alpha> (of_cnf ([P \<phi>] # tseitin \<phi>)))"
+ "(\<exists>\<alpha>. eval \<alpha> (of_cnf ([P \<phi>] # tseitin2 \<phi> []))) 
+  \<longleftrightarrow> (\<exists>\<alpha>. eval \<alpha> (of_cnf ([P \<phi>] # tseitin \<phi>)))"
 proof -
   have 1: "\<forall>\<alpha>. eval \<alpha> (of_cnf(tseitin2 \<phi> [])) \<longleftrightarrow> eval \<alpha> (of_cnf(tseitin \<phi>))" 
     by (rule tseitin_eq_for_all)
@@ -396,17 +428,24 @@ proof -
     assume 2: "\<exists>\<alpha>. eval \<alpha> (of_cnf ([P \<phi>] # tseitin2 \<phi> []))"
     show "\<exists>\<alpha>. eval \<alpha> (of_cnf ([P \<phi>] # tseitin \<phi>))"
     proof -
-      from 2 obtain \<alpha> where 3: "\<alpha> \<phi>" and 4: "eval \<alpha> (of_cnf (tseitin2 \<phi> []))" by auto
-      from 1 have "eval \<alpha> (of_cnf(tseitin2 \<phi> [])) \<longleftrightarrow> eval \<alpha> (of_cnf(tseitin \<phi>))" by (rule allE)
+      from 2 obtain \<alpha> where 3: "\<alpha> \<phi>" and 4: "eval \<alpha> (of_cnf (tseitin2 \<phi> []))" 
+        by auto
+      from 1 have 
+        "eval \<alpha> (of_cnf(tseitin2 \<phi> [])) \<longleftrightarrow> eval \<alpha> (of_cnf(tseitin \<phi>))" 
+        by (rule allE)
       from this and 3 and 4 show ?thesis by auto
     qed
     next
       assume 5: "\<exists>\<alpha>. eval \<alpha> (of_cnf ([P \<phi>] # tseitin \<phi>))"
       show "\<exists>\<alpha>. eval \<alpha> (of_cnf ([P \<phi>] # tseitin2 \<phi> []))"
       proof -
-      from 5 obtain \<alpha> where 6: "\<alpha> \<phi>" and 7: "eval \<alpha> (of_cnf (tseitin \<phi>))" by auto
-      from 1 have "eval \<alpha> (of_cnf(tseitin2 \<phi> [])) \<longleftrightarrow> eval \<alpha> (of_cnf(tseitin \<phi>))" by (rule allE)
-      then have "eval \<alpha> (of_cnf(tseitin \<phi>)) \<longleftrightarrow> eval \<alpha> (of_cnf(tseitin2 \<phi> []))" by (rule sym)
+        from 5 obtain \<alpha> where 6: "\<alpha> \<phi>" and 7: "eval \<alpha> (of_cnf (tseitin \<phi>))" 
+          by auto
+        from 1 have 
+          "eval \<alpha> (of_cnf(tseitin2 \<phi> [])) \<longleftrightarrow> eval \<alpha> (of_cnf(tseitin \<phi>))" 
+          by (rule allE)
+        then have "eval \<alpha> (of_cnf(tseitin \<phi>)) \<longleftrightarrow> eval \<alpha> (of_cnf(tseitin2 \<phi> []))" 
+          by (rule sym)
       from this and 6 and 7 show ?thesis by auto
     qed
   qed
@@ -418,9 +457,11 @@ Finally we prove that \<open>a\<^sub>\<phi> \<and> tseitin2 \<phi>\<close> and \
 lemma tseitin2_equisat:
   "sat (of_cnf ([P \<phi>] # tseitin2 \<phi> [])) \<longleftrightarrow> sat \<phi>"
 proof -
-  have "sat (of_cnf ([P \<phi>] # tseitin2 \<phi> [])) \<longleftrightarrow> (\<exists>\<alpha>. eval \<alpha> (of_cnf ([P \<phi>] # tseitin2 \<phi> [])))" 
+  have "sat (of_cnf ([P \<phi>] # tseitin2 \<phi> [])) 
+    \<longleftrightarrow> (\<exists>\<alpha>. eval \<alpha> (of_cnf ([P \<phi>] # tseitin2 \<phi> [])))" 
     unfolding sat_def ..
-  also have "... \<longleftrightarrow> (\<exists>\<alpha>. eval \<alpha> (of_cnf ([P \<phi>] # tseitin \<phi>)))" unfolding tseitin_eq_ex ..
+  also have "... \<longleftrightarrow> (\<exists>\<alpha>. eval \<alpha> (of_cnf ([P \<phi>] # tseitin \<phi>)))" 
+    unfolding tseitin_eq_ex ..
   also have "... \<longleftrightarrow> sat (of_cnf ([P \<phi>] # tseitin \<phi>))" unfolding sat_def ..
   also have "... \<longleftrightarrow> sat \<phi>" unfolding tseitin_equisat ..
   finally show ?thesis by auto
@@ -445,18 +486,20 @@ fun plaisted :: "bool \<Rightarrow> 'a form \<Rightarrow> ('a form) cnf"
   | "plaisted True (Neg \<phi>) = [(N (Neg \<phi>)), (N \<phi>)] # plaisted False \<phi>"
   | "plaisted False (Neg \<phi>) = [(P (Neg \<phi>)), (P \<phi>)] # plaisted True \<phi>"
   | "plaisted True (Imp \<phi> \<psi>) = [(N (Imp \<phi> \<psi>)), (N \<phi>), (P \<psi>)] 
-                                # (plaisted False \<phi> @ plaisted True \<psi>)"
-  | "plaisted False (Imp \<phi> \<psi>) = [(P (Imp \<phi> \<psi>)), (P \<phi>)] # [(N \<psi>), (P (Imp \<phi> \<psi>))]
-                                # (plaisted True \<phi> @ plaisted False \<psi>)"
+    # (plaisted False \<phi> @ plaisted True \<psi>)"
+  | "plaisted False (Imp \<phi> \<psi>) = [(P (Imp \<phi> \<psi>)), (P \<phi>)] 
+    # [(N \<psi>), (P (Imp \<phi> \<psi>))] # (plaisted True \<phi> @ plaisted False \<psi>)"
 
 text \<open>
 We show two auxiliary lemmas:
 \<close>
 lemma [simp]: 
-  "eval (eval \<alpha>) (of_cnf(plaisted True \<phi>)) \<longleftrightarrow> eval (eval \<alpha>) (of_cnf(plaisted False \<phi>))"
+  "eval (eval \<alpha>) (of_cnf(plaisted True \<phi>)) 
+    \<longleftrightarrow> eval (eval \<alpha>) (of_cnf(plaisted False \<phi>))"
   by (induction \<phi>) auto
 
-lemma [simp]: "eval (eval \<alpha>) (of_cnf(plaisted p \<phi>))"
+lemma [simp]: 
+  "eval (eval \<alpha>) (of_cnf(plaisted p \<phi>))"
 proof (cases p)
   case True
   then show ?thesis by (induction \<phi>) auto
@@ -467,10 +510,11 @@ qed
 
 text \<open>
 We show that the structure preserving translation to clause form is consistency preserving 
-for {@const plaisted}.
+for @{const plaisted}.
 \<close>
-lemma plaisted_consistent: "(\<alpha> \<phi> \<and> eval \<alpha> (of_cnf(plaisted True \<phi>)) \<longrightarrow> eval (\<alpha> \<circ> Atm) \<phi>)
-          \<and> ((\<not>\<alpha> \<phi>) \<and> eval \<alpha> (of_cnf(plaisted False \<phi>)) \<longrightarrow> (\<not>eval (\<alpha> \<circ> Atm) \<phi>))"
+lemma plaisted_consistent: 
+    "(\<alpha> \<phi> \<and> eval \<alpha> (of_cnf(plaisted True \<phi>)) \<longrightarrow> eval (\<alpha> \<circ> Atm) \<phi>)
+     \<and> ((\<not>\<alpha> \<phi>) \<and> eval \<alpha> (of_cnf(plaisted False \<phi>)) \<longrightarrow> (\<not>eval (\<alpha> \<circ> Atm) \<phi>))"
   by (induction \<phi>) auto
 
 text \<open>
@@ -482,13 +526,15 @@ proof (rule iffI)
   assume 1: "sat (of_cnf ([P \<phi>] # plaisted True \<phi>))"
   show "sat \<phi>"
   proof -
-    from 1 have "\<exists>\<alpha>. eval \<alpha> (of_cnf ([P \<phi>] # plaisted True \<phi>))" by (simp add: sat_def)
+    from 1 have "\<exists>\<alpha>. eval \<alpha> (of_cnf ([P \<phi>] # plaisted True \<phi>))" 
+      by (simp add: sat_def)
     then have "\<exists>\<alpha>. (\<alpha> \<phi>) \<and> eval \<alpha> (of_cnf (plaisted True \<phi>))" by auto
     then obtain \<alpha> where 2: "\<alpha> \<phi> \<and> eval \<alpha> (of_cnf (plaisted True \<phi>))" by auto
     have "(\<alpha> \<phi> \<and> eval \<alpha> (of_cnf(plaisted True \<phi>)) \<longrightarrow> eval (\<alpha> \<circ> Atm) \<phi>)
-          \<and> ((\<not>\<alpha> \<phi>) \<and> eval \<alpha> (of_cnf(plaisted False \<phi>)) \<longrightarrow> (\<not>eval (\<alpha> \<circ> Atm) \<phi>))" 
+      \<and> ((\<not>\<alpha> \<phi>) \<and> eval \<alpha> (of_cnf(plaisted False \<phi>)) \<longrightarrow> (\<not>eval (\<alpha> \<circ> Atm) \<phi>))" 
       by (rule plaisted_consistent)
-    then have "(\<alpha> \<phi> \<and> eval \<alpha> (of_cnf(plaisted True \<phi>)) \<longrightarrow> eval (\<alpha> \<circ> Atm) \<phi>)" by auto
+    then have "(\<alpha> \<phi> \<and> eval \<alpha> (of_cnf(plaisted True \<phi>)) \<longrightarrow> eval (\<alpha> \<circ> Atm) \<phi>)" 
+      by auto
     from this and 2 have "eval (\<alpha> \<circ> Atm) \<phi>" by (rule mp)
     then have "\<exists>\<beta>. eval \<beta> \<phi>" by auto
     then show ?thesis by (simp add: sat_def)
@@ -505,7 +551,7 @@ next
 qed
 
 text \<open>
-We prove linear bounds on the number of clauses of {@const plaisted}:
+We prove linear bounds on the number of clauses of @{const plaisted}:
 \<close>
 lemma plaisted_num_clauses:
   "length (plaisted p \<phi>) \<le> 2 * size \<phi>"
@@ -517,12 +563,14 @@ next
   then show ?case by auto
 next
   case IH: (Neg \<phi>)
-  have "length (plaisted p (Neg \<phi>)) = 1 + length (plaisted (\<not>p) \<phi>)" by (cases p) auto
+  have "length (plaisted p (Neg \<phi>)) = 1 + length (plaisted (\<not>p) \<phi>)" 
+    by (cases p) auto
   also have "... \<le> 1 + 2 * size \<phi>" using IH by auto 
   finally show ?case by auto
 next
   case IH: (Imp \<phi> \<psi>)
-  have "length (plaisted p (Imp \<phi> \<psi>)) \<le> 2 + length (plaisted (\<not>p) \<phi>) + length (plaisted p \<psi>)"
+  have "length (plaisted p (Imp \<phi> \<psi>)) 
+    \<le> 2 + length (plaisted (\<not>p) \<phi>) + length (plaisted p \<psi>)"
     by (cases p) auto
   also have "... \<le> 2 + length (plaisted (\<not>p) \<phi>) + 2 * size \<psi>"
     using IH by auto
@@ -532,7 +580,7 @@ next
 qed
 
 text \<open>
-We show a linear bound on the number of literals for {@const plaisted}.
+We show a linear bound on the number of literals for @{const plaisted}.
 \<close>
 lemma plaisted_num_literals:
   "num_literals (plaisted p \<phi>) \<le> 4 * size \<phi>"
@@ -544,7 +592,8 @@ next
   then show ?case by auto
 next
   case IH: (Neg \<phi>)
-  have "num_literals (plaisted p (Neg \<phi>)) = 2 + num_literals (plaisted (\<not>p) \<phi>)" by (cases p) auto
+  have "num_literals (plaisted p (Neg \<phi>)) = 2 + num_literals (plaisted (\<not>p) \<phi>)" 
+    by (cases p) auto
   also have "... \<le> 2 + 4 * size \<phi>" using IH by auto 
   finally show ?case by auto
 next
@@ -573,15 +622,19 @@ next
   then show ?case by auto
 next
   case IH: (Neg \<phi>)
-  have "length (plaisted p (Neg \<phi>)) = 1 + length (plaisted (\<not>p) \<phi>)" by (cases p) auto
+  have "length (plaisted p (Neg \<phi>)) = 1 + length (plaisted (\<not>p) \<phi>)" 
+    by (cases p) auto
   also have "... \<le> 1 + length (tseitin \<phi>)" using IH by auto
   finally show ?case by auto
 next
   case IH: (Imp \<phi> \<psi>)
-  have "length (plaisted p (Imp \<phi> \<psi>)) \<le> 2 + length (plaisted (\<not>p) \<phi>) + length (plaisted p \<psi>)"
+  have "length (plaisted p (Imp \<phi> \<psi>)) 
+    \<le> 2 + length (plaisted (\<not>p) \<phi>) + length (plaisted p \<psi>)"
     by (cases p) auto
-  also have "... \<le> 2 + length (plaisted (\<not>p) \<phi>) + length (tseitin \<psi>)" using IH by auto
-  also have "... \<le> 2 + length (tseitin \<phi>) + length (tseitin \<psi>)" using IH by auto
+  also have "... \<le> 2 + length (plaisted (\<not>p) \<phi>) + length (tseitin \<psi>)" 
+    using IH by auto
+  also have "... \<le> 2 + length (tseitin \<phi>) + length (tseitin \<psi>)" 
+    using IH by auto
   finally show ?case by auto
 qed
 
@@ -595,7 +648,8 @@ next
   then show ?case by auto
 next
   case IH: (Neg \<phi>)
-  have "num_literals (plaisted p (Neg \<phi>)) = 2 + num_literals (plaisted (\<not>p) \<phi>)" by (cases p) auto
+  have "num_literals (plaisted p (Neg \<phi>)) = 2 + num_literals (plaisted (\<not>p) \<phi>)"
+    by (cases p) auto
   also have "... \<le> 2 + num_literals (tseitin \<phi>)" using IH by auto
   finally show ?case by auto
 next
@@ -603,8 +657,10 @@ next
   have "num_literals (plaisted p (Imp \<phi> \<psi>)) 
           \<le> 4 + num_literals (plaisted (\<not>p) \<phi>) + num_literals (plaisted p \<psi>)"
     by (cases p) auto
-  also have "... \<le> 4 + num_literals (plaisted (\<not>p) \<phi>) + num_literals (tseitin \<psi>)" using IH by auto
-  also have "... \<le> 4 + num_literals (tseitin \<phi>) + num_literals (tseitin \<psi>)" using IH by auto
+  also have "... \<le> 4 + num_literals (plaisted (\<not>p) \<phi>) + num_literals (tseitin \<psi>)" 
+    using IH by auto
+  also have "... \<le> 4 + num_literals (tseitin \<phi>) + num_literals (tseitin \<psi>)" 
+    using IH by auto
   finally show ?case by auto
 qed
 
