ROOT
@@ -1,10 +1,6 @@
 session project_tseitin = HOL +
   options [document = pdf, document_output = "output"]
-(*theories [document = false]
-    A
-    B
-  theories
-    C
-    D*)
+theories
+Project_Tseitin
   document_files
     "root.tex"
